allocator/slabs bottom-up 2/n
move axiomatized utils apart

alloc/Slabs.fst
@@ -18,19 +18,7 @@ open Seq2
 let array = Steel.ST.Array.array
 let ptr = Steel.ST.Array.ptr
 
-open Bitmap5
-
-let slab_region_len : U64.t = 16777216UL
-
-let slab_region = r:array U8.t{A.length r = U64.v slab_region_len}
-
-assume val get_slab_region (_:unit)
-  : slab_region
-
-let slab_metadata = r:array U64.t{A.length r = 4}
-
-assume val get_slab_metadata (_:unit)
-  : slab_metadata
+open Utils
 
 assume val get_free_slot (ptr_md: slab_metadata)
   : Steel U32.t
@@ -58,7 +46,7 @@ let allocate_small (len: U32.t) (md: slab_metadata)
   =
   let a = get_slab_region () in
   let slot = get_free_slot md in
-  bm_set #4 md slot;
+  Bitmap5.bm_set #4 md slot;
   let offset = U32.mul 32ul slot in
   let ptr_slab_region = A.ptr_of a in
   let ptr = A.ptr_shift ptr_slab_region offset in
