alloc/Utils.fst
@@ -1,0 +1,54 @@
+module Utils
+
+module U64 = FStar.UInt64
+module U32 = FStar.UInt32
+module I32 = FStar.Int32
+module U8 = FStar.UInt8
+
+open Steel.Effect.Atomic
+open Steel.Effect
+module A = Steel.Array
+
+let array = Steel.ST.Array.array
+let ptr = Steel.ST.Array.ptr
+
+// 1) ptr_diff_t
+assume val ptrdiff (arr1 arr2: array U8.t)
+  : Steel I32.t
+  (A.varray arr1 `star` A.varray arr2)
+  (fun _ -> A.varray arr1 `star` A.varray arr2)
+  (requires fun h0 ->
+    let ptr1 = A.ptr_of arr1 in
+    let ptr2 = A.ptr_of arr2 in
+    A.base ptr1 == A.base ptr2)
+  (ensures fun h0 r h1 ->
+    let ptr1 = A.ptr_of arr1 in
+    let ptr2 = A.ptr_of arr2 in
+    A.asel arr1 h1 == A.asel arr1 h0 /\
+    A.asel arr2 h1 == A.asel arr2 h0 /\
+    I32.v r == A.offset ptr2 - A.offset ptr1
+  )
+
+// 2) ffs64/ffz64
+open Bitmap5
+assume val ffs64 (x: U64.t)
+  : Pure U32.t
+  (requires U64.v x > 0)
+  (ensures fun r ->
+    U32.v r < 64 /\
+    FStar.UInt.nth (U64.v x) (U32.v r) = true
+  )
+
+let slab_region_len : U64.t = 16777216UL
+
+let slab_region = r:array U8.t{A.length r = U64.v slab_region_len}
+
+// C binding, no top-level Steel initialization
+assume val get_slab_region (_:unit)
+  : slab_region
+
+let slab_metadata = r:array U64.t{A.length r = 4}
+
+// C binding, no top-level Steel initialization
+assume val get_slab_metadata (_:unit)
+  : slab_metadata
